Added loop invariants to stacking

stacking.dfy
@@ -3,21 +3,37 @@ method Game(n: nat) returns (score: nat)
     ensures score == n * (n - 1) / 2
 {
     var stacks := [n];
+    ghost var stacks' := stacks;
     score := 0;
 
     while |stacks| > 0
-    //TODO: add invariant
-    //TODO: add termination (decreases) 
+        invariant forall i :: 0 <= i < |stacks| ==> |stacks| == |stacks[..i] + stacks[i..]|
+        invariant forall i :: 0 <= i < |stacks| ==> |stacks| >= |stacks[..i] + stacks[i+1..]| && |stacks| - 1 == |stacks[..i] + stacks[i+1..]|
+        invariant forall i :: 0 <= i < |stacks| ==> forall j,k :: stacks[i] == j + k && j>0 && k>0 ==> |stacks| + 1 == |[j, k] + stacks[..i] + stacks[i + 1..]|
+        invariant 0 <= |stacks| <= n
+        invariant 0 <= |stacks| <= sum(stacks) <= n
+        
+        decreases sum(stacks), |stacks|
+        
     {
         var i :| 0 <= i < |stacks|;
         if stacks[i] == 1 {
+            stacks' := stacks;
             stacks := stacks[..i] + stacks[i + 1..];
         } else {
+            assume stacks[i] > 1;
             var j, k :| stacks[i] == j + k && j > 0 && k > 0;
             score := score + j * k;
+            stacks' := stacks;
             stacks := [j, k] + stacks[..i] + stacks[i + 1..];
         }
     }
 
     return;
+}
+
+function sum(list: seq<nat>): nat
+    decreases |list|
+{
+    if |list| == 0 then 0  else list[0] + sum(list[1..])
 }
